Enable String case of EqualConst

compiler/backend/semantics/bvlSemScript.sml
@@ -295,6 +295,11 @@ val do_app_def = Define `
         (case p of
          | Int i => (case x1 of Number j => Rval (Boolv (i = j), s) | _ => Error)
          | W64 i => (case x1 of Word64 j => Rval (Boolv (i = j), s) | _ => Error)
+         | Str i => (case x1 of RefPtr p =>
+                       (case FLOOKUP s.refs p of SOME (ByteArray T j) =>
+                          Rval (Boolv (j = MAP (n2w ∘ ORD) (explode i)), s)
+                        | _ => Error)
+                     | _ => Error)
          | _ => Error)
     | (Equal,[x1;x2]) =>
         (case do_eq s.refs x1 x2 of
